proof/AdequacyLocal.v
@@ -20,15 +20,6 @@ Set Implicit Arguments.
 
 
 
-(* TODO: move to coqlibc *)
-Ltac revert_until_bar :=
-  on_last_hyp ltac:(fun id' => match (type of id') with
-                               | bar_True => idtac
-                               | _ => revert id'; revert_until_bar
-                               end)
-.
-
-Ltac folder := all_once_fast ltac:(fun H => try (is_local_definition H; fold_all H)).
 
 
 
@@ -57,6 +48,7 @@ Section SIMGE.
       msps
       (SIMSKENV: List.Forall (fun msp => ModSemPair.sim_skenv msp sm0) msps)
       (SIMMSS: List.Forall (ModSemPair.sim) msps)
+      (MFUTURE: List.Forall (fun msp => SimMem.future msp.(ModSemPair.sm) sm0) msps)
       ge_src ge_tgt
       (GESRC: ge_src = (map (ModSemPair.src) msps))
       (GETGT: ge_tgt = (map (ModSemPair.tgt) msps))
@@ -88,6 +80,7 @@ Section SIMGE.
     :
       exists msp,
         <<SRC: msp.(ModSemPair.src) = ms_src>>
+        /\ <<MFUTURE: SimMem.future msp.(ModSemPair.sm) sm0>>
         /\ <<FINDTGT: Ge.find_fptr_owner ge_tgt fptr_tgt msp.(ModSemPair.tgt)>>
         /\ <<SIMMS: ModSemPair.sim msp>>
         /\ <<SIMSKENV: ModSemPair.sim_skenv msp sm0>>
@@ -141,9 +134,12 @@ Section SIMGE.
     inv SIMGE.
     { econs; eauto. }
     econs 2; try reflexivity; eauto.
-    rewrite Forall_forall in *. ii.
-    eapply SimSymb.mle_preserves_sim_skenv; eauto.
-    eapply SIMSKENV; eauto.
+    - rewrite Forall_forall in *. ii.
+      eapply SimSymb.mle_preserves_sim_skenv; eauto.
+      eapply SIMSKENV; eauto.
+    - rewrite Forall_forall in *. ii.
+      etrans; try apply MFUTURE; eauto.
+      econs; try left; eauto.
   Qed.
 
   Theorem mlift_preserves_sim_ge
@@ -157,10 +153,13 @@ Section SIMGE.
     inv SIMGE.
     { econs; eauto. }
     econs 2; try reflexivity; eauto.
-    rewrite Forall_forall in *. ii.
-    u.
-    eapply SimSymb.mlift_preserves_sim_skenv; eauto.
-    eapply SIMSKENV; eauto.
+    - rewrite Forall_forall in *. ii.
+      u.
+      eapply SimSymb.mlift_preserves_sim_skenv; eauto.
+      eapply SIMSKENV; eauto.
+    - rewrite Forall_forall in *. ii.
+      etrans; try apply MFUTURE; eauto.
+      econs; try right; eauto.
   Qed.
 
   (* Lemma load_modsems_sim_ge_aux *)
@@ -193,12 +192,13 @@ Section SIMGE.
     inv SIMGEHD. destruct msps; ss. destruct msps; ss. clarify. inv SIMMSS. inv SIMSKENV.
     inv SIMGETL; ss.
     econstructor 2 with (msps := t :: msps); eauto.
+    inv MFUTURE. econs; eauto.
   Qed.
 
   Lemma to_msp_tgt
-        skenv_tgt skenv_src pp
+        skenv_tgt skenv_src sm pp
     :
-          map ModSemPair.tgt (map (ModPair.to_msp skenv_src skenv_tgt) pp) =
+          map ModSemPair.tgt (map (ModPair.to_msp skenv_src skenv_tgt sm) pp) =
           map (fun md => Mod.modsem md skenv_tgt) (ProgPair.tgt pp)
   .
   Proof.
@@ -207,9 +207,9 @@ Section SIMGE.
   Qed.
 
   Lemma to_msp_src
-        skenv_tgt skenv_src pp
+        skenv_tgt skenv_src sm pp
     :
-          map ModSemPair.src (map (ModPair.to_msp skenv_src skenv_tgt) pp) =
+          map ModSemPair.src (map (ModPair.to_msp skenv_src skenv_tgt sm) pp) =
           map (fun md => Mod.modsem md skenv_src) (ProgPair.src pp)
   .
   Proof.
@@ -227,7 +227,7 @@ Section SIMGE.
                           (Mod.get_sk (ModPair.tgt mp) (Mod.data (ModPair.tgt mp))) ss_link)
         (SIMSKENV: SimSymb.sim_skenv sm_init ss_link skenv_src skenv_tgt)
       :
-        <<SIMSKENV: ModSemPair.sim_skenv (ModPair.to_msp skenv_src skenv_tgt mp) sm_init>>
+        <<SIMSKENV: ModSemPair.sim_skenv (ModPair.to_msp skenv_src skenv_tgt sm_init mp) sm_init>>
   .
   Proof.
     (* inv SIMMP. specialize (SIMMS skenv_src skenv_tgt). *)
@@ -279,10 +279,12 @@ Section SIMGE.
     - assert(exists msp_sys,
                 (<<SYSSRC: msp_sys.(ModSemPair.src) = System.modsem (Genv.globalenv sk_link_src)>>)
                 /\ (<<SYSTGT: msp_sys.(ModSemPair.tgt) = System.modsem (Genv.globalenv sk_link_tgt)>>)
+                /\ (<<SYSSM: msp_sys.(ModSemPair.sm) = sm_init>>)
                 /\ <<SYSSIM: ModSemPair.sim msp_sys>> /\ <<SIMSKENV: ModSemPair.sim_skenv msp_sys sm_init>>).
       { admit "raw admit. this should hold.". }
       des.
       econstructor 2 with (msps := [msp_sys]); ss; eauto.
+      + econs; eauto. eapply rtc_once. clarify. left. refl.
       + rewrite SYSSRC. ss.
       + rewrite SYSTGT. ss.
     - ginduction pp; ii; ss.
@@ -301,9 +303,13 @@ Section SIMGE.
       assert(WFTGT: SkEnv.wf skenv_tgt).
       { eapply Sk.load_skenv_wf. }
       econstructor 2 with
-          (msps := (map (ModPair.to_msp skenv_src skenv_tgt) (mp :: pp))); eauto; revgoals.
+          (msps := (map (ModPair.to_msp skenv_src skenv_tgt sm_init) (mp :: pp))); eauto; revgoals.
       + ss. f_equal. rewrite to_msp_tgt; ss.
       + ss. f_equal. rewrite to_msp_src; ss.
+      + ss. econs; eauto.
+        rewrite Forall_forall in *.
+        i. apply in_map_iff in H. des.
+        clarify. ss. reflexivity.
       + ss. econs; ss; eauto.
         * eapply SIMMP; eauto.
         * rewrite Forall_forall in *.
